removed sort annotations from contexts in definitions

theories/Core/Syntactic/System/Definitions.v
@@ -16,21 +16,21 @@ Reserved Notation "Γ ⊢s σ : Δ" (in custom judg at level 80, Γ custom exp, 
 Reserved Notation "Γ ⊢s σ ≈ σ' : Δ" (in custom judg at level 80, Γ custom exp, σ custom exp, σ' custom exp, Δ custom exp).
 Reserved Notation "⊢ Γ ⊆ Γ'" (in custom judg at level 80, Γ custom exp, Γ' custom exp).
 Reserved Notation "Γ ⊢ A ⊆ A'" (in custom judg at level 80, Γ custom exp, A custom exp, A' custom exp).
-Reserved Notation "'#' x : A @ s ∈ Γ" (in custom judg at level 80, x constr at level 0, A custom exp, s custom exp, Γ custom exp at level 50).
+Reserved Notation "'#' x : A ∈ Γ" (in custom judg at level 80, x constr at level 0, A custom exp, Γ custom exp at level 50).
 
 Generalizable All Variables.
 
-Inductive ctx_lookup {P : PtsSig} : nat -> typ P -> P -> ctx P -> Prop :=
-  | here : `({{ #0 : A[Wk]@s ∈ Γ, A@s }})
-  | there : `({{ #n : A@s ∈ Γ }} -> {{ #(S n) : A[Wk]@s ∈ Γ, B@s' }})
-where "'#' x : A @ K ∈ Γ" := (ctx_lookup x A K Γ) (in custom judg) : type_scope.
+Inductive ctx_lookup {P : PtsSig} : nat -> typ P -> ctx P -> Prop :=
+  | here : `({{ #0 : A[Wk] ∈ Γ, A }})
+  | there : `({{ #n : A ∈ Γ }} -> {{ #(S n) : A[Wk] ∈ Γ, B }})
+where "'#' x : A ∈ Γ" := (ctx_lookup x A Γ) (in custom judg) : type_scope.
 
 Inductive wf_ctx {P : PtsSig} : ctx P -> Prop :=
 | wf_ctx_empty : {{ ⊢ ⋅ }}
 | wf_ctx_extend :
   `( {{ ⊢ Γ }} ->
      {{ Γ ⊢ A : Sort@s }} ->
-     {{ ⊢ Γ, A@s }} )
+     {{ ⊢ Γ, A }} )
 where "⊢ Γ" := (wf_ctx Γ) (in custom judg) : type_scope
 
 with wf_ctx_sub {P : PtsSig} : ctx P -> ctx P -> Prop :=
@@ -40,7 +40,7 @@ with wf_ctx_sub {P : PtsSig} : ctx P -> ctx P -> Prop :=
      {{ Γ ⊢ A : Sort@s }} ->
      {{ Δ ⊢ A' : Sort@s }} ->
      {{ Γ ⊢ A ⊆ A' }} ->
-     {{ ⊢ Γ, A@s ⊆ Δ, A'@s }} )
+     {{ ⊢ Γ, A ⊆ Δ, A' }} )
 where "⊢ Γ ⊆ Γ'" := (wf_ctx_sub Γ Γ') (in custom judg) : type_scope
                                                            
 with wf_exp {P : PtsSig} : ctx P -> typ P -> exp P -> Prop :=
@@ -53,18 +53,18 @@ with wf_exp {P : PtsSig} : ctx P -> typ P -> exp P -> Prop :=
 | wf_pi :
   `( forall (r : Ru_pi P s1 s2 s3),
       {{ Γ ⊢ A : Sort@s1 }} ->
-      {{ Γ, A@s1 ⊢ B : Sort@s2 }} ->
+      {{ Γ, A ⊢ B : Sort@s2 }} ->
       {{ Γ ⊢ Π r A B : Sort@s3 }} )
 | wf_fn :
   `( forall (r : Ru_pi P s1 s2 s3),
         {{ Γ ⊢ A : Sort@s1 }} ->
-        {{ Γ, A@s1 ⊢ B : Sort@s2 }} ->
-        {{ Γ, A@s1 ⊢ M : B }} ->
+        {{ Γ, A ⊢ B : Sort@s2 }} ->
+        {{ Γ, A ⊢ M : B }} ->
         {{ Γ ⊢ λ r A B M : Π r A B }} )
 | wf_app :
   `( forall (r : Ru_pi P s1 s2 s3),
         {{ Γ ⊢ A : Sort@s1 }} ->
-        {{ Γ, A@s1 ⊢ B : Sort@s2 }} ->
+        {{ Γ, A ⊢ B : Sort@s2 }} ->
         {{ Γ ⊢ M : Π r A B }} ->
         {{ Γ ⊢ N : A }} ->
         {{ Γ ⊢ M N : B[Id,,N] }} )
@@ -73,7 +73,7 @@ with wf_exp {P : PtsSig} : ctx P -> typ P -> exp P -> Prop :=
   `( {{ ⊢ Γ }} ->
      (** This premise is redundant, but helpful for soundness *)
      {{ Γ ⊢ A : Sort@s }} ->
-     {{ #x : A@s ∈ Γ }} ->
+     {{ #x : A ∈ Γ }} ->
      {{ Γ ⊢ #x : A }} )
 
 (** Naturals **)
@@ -91,9 +91,9 @@ with wf_exp {P : PtsSig} : ctx P -> typ P -> exp P -> Prop :=
         {{ Γ ⊢ succ M : ℕ}} )
 | wf_natrec :
   `( forall (r : Ru_nat P s),
-        {{ Γ, ℕ@s ⊢ A : Sort@s' }} ->
+        {{ Γ, ℕ ⊢ A : Sort@s' }} ->
         {{ Γ ⊢ MZ : A[Id,,zero] }} ->
-        {{ Γ, ℕ@s, A@s' ⊢ MS : A[Wk∘Wk,,succ #1] }} ->
+        {{ Γ, ℕ, A ⊢ MS : A[Wk∘Wk,,succ #1] }} ->
         {{ Γ ⊢ M : ℕ}} ->
         {{ Γ ⊢ rec M return A | zero -> MZ | succ -> MS end : A[Id,,M] }} )
 
@@ -118,8 +118,8 @@ with wf_sub {P : PtsSig} : ctx P -> ctx P -> sub P -> Prop :=
   `( {{ ⊢ Γ }} ->
      {{ Γ ⊢s Id : Γ }} )
 | wf_sub_weaken :
-  `( {{ ⊢ Γ, A@s }} ->
-     {{ Γ, A@s ⊢s Wk : Γ }} )
+  `( {{ ⊢ Γ, A }} ->
+     {{ Γ, A ⊢s Wk : Γ }} )
 | wf_sub_compose :
   `( {{ Γ1 ⊢s σ2 : Γ2 }} ->
      {{ Γ2 ⊢s σ1 : Γ3 }} ->
@@ -128,7 +128,7 @@ with wf_sub {P : PtsSig} : ctx P -> ctx P -> sub P -> Prop :=
   `( {{ Γ ⊢s σ : Δ }} ->
      {{ Δ ⊢ A : Sort@s }} ->
      {{ Γ ⊢ M : A[σ] }} ->
-     {{ Γ ⊢s σ,,M : Δ, A@s }} )
+     {{ Γ ⊢s σ,,M : Δ, A }} )
 | wf_sub_conv :
   `( {{ Γ ⊢s σ : Δ }} ->
      (** As in [wf_exp_conv], we need this extra argument for soundness *)
@@ -147,7 +147,7 @@ with wf_ctx_eq {P : PtsSig} : ctx P -> ctx P -> Prop :=
      {{ Δ ⊢ A' : Sort@s }} ->
      {{ Γ ⊢ A ≈ A' : Sort@s }} ->
      {{ Δ ⊢ A ≈ A' : Sort@s }} ->
-     {{ ⊢ Γ, A@s ≈ Δ, A'@s }} )
+     {{ ⊢ Γ, A ≈ Δ, A' }} )
 where "⊢ Γ ≈ Γ'" := (wf_ctx_eq Γ Γ') (in custom judg) : type_scope
 
 with wf_exp_eq {P : PtsSig} : ctx P -> typ P -> exp P -> exp P -> Prop :=
@@ -161,33 +161,33 @@ with wf_exp_eq {P : PtsSig} : ctx P -> typ P -> exp P -> exp P -> Prop :=
   `( forall (r : Ru_pi P s1 s2 s3),
         {{ Γ ⊢s σ : Δ }} ->
         {{ Δ ⊢ A : Sort@s1 }} ->
-        {{ Δ, A@s1 ⊢ B : Sort@s2 }} ->
+        {{ Δ, A ⊢ B : Sort@s2 }} ->
         {{ Γ ⊢ (Π r A B)[σ] ≈ Π r A[σ] B[q σ] : Sort@s3 }} )
 | wf_exp_eq_pi_cong :
   `( forall (r : Ru_pi P s1 s2 s3),
         {{ Γ ⊢ A : Sort@s1 }} ->
         {{ Γ ⊢ A ≈ A' : Sort@s1 }} ->
-        {{ Γ, A@s1 ⊢ B ≈ B' : Sort@s2 }} ->
+        {{ Γ, A ⊢ B ≈ B' : Sort@s2 }} ->
         {{ Γ ⊢ Π r A B ≈ Π r A' B' : Sort@s3 }} )
 | wf_exp_eq_fn_cong :
   `( forall (r : Ru_pi P s1 s2 s3),
         {{ Γ ⊢ A : Sort@s1 }} ->
         {{ Γ ⊢ A ≈ A' : Sort@s1 }} ->
-        {{ Γ, A@s1 ⊢ B : Sort@s2 }} ->
-        {{ Γ, A@s1 ⊢ B ≈ B' : Sort@s2 }} ->
-        {{ Γ, A@s1 ⊢ M ≈ M' : B }} ->
+        {{ Γ, A ⊢ B : Sort@s2 }} ->
+        {{ Γ, A ⊢ B ≈ B' : Sort@s2 }} ->
+        {{ Γ, A ⊢ M ≈ M' : B }} ->
         {{ Γ ⊢ λ r A B M ≈ λ r A' B' M' : Π r A B }} )
 | wf_exp_eq_fn_sub :
   `( forall (r : Ru_pi P s1 s2 s3),
         {{ Γ ⊢s σ : Δ }} ->
         {{ Δ ⊢ A : Sort@s1 }} ->
-        {{ Δ, A@s1 ⊢ B : Sort@s2 }} ->
-        {{ Δ, A@s1 ⊢ M : B }} ->
+        {{ Δ, A ⊢ B : Sort@s2 }} ->
+        {{ Δ, A ⊢ M : B }} ->
         {{ Γ ⊢ (λ r A B M)[σ] ≈ λ r A[σ] B[q σ] M[q σ] : (Π r A B)[σ] }} )
 | wf_exp_eq_app_cong :
   `( forall (r : Ru_pi P s1 s2 s3),
         {{ Γ ⊢ A : Sort@s1 }} ->
-        {{ Γ, A@s1 ⊢ B : Sort@s2 }} ->
+        {{ Γ, A ⊢ B : Sort@s2 }} ->
         {{ Γ ⊢ M ≈ M' : Π r A B }} ->
         {{ Γ ⊢ N ≈ N' : A }} ->
         {{ Γ ⊢ M N ≈ M' N' : B[Id,,N] }} )
@@ -195,21 +195,21 @@ with wf_exp_eq {P : PtsSig} : ctx P -> typ P -> exp P -> exp P -> Prop :=
   `( forall (r : Ru_pi P s1 s2 s3),
         {{ Γ ⊢s σ : Δ }} ->
         {{ Δ ⊢ A : Sort@s1 }} ->
-        {{ Δ, A@s1 ⊢ B : Sort@s2 }} ->
+        {{ Δ, A ⊢ B : Sort@s2 }} ->
         {{ Δ ⊢ M : Π r A B }} ->
         {{ Δ ⊢ N : A }} ->
         {{ Γ ⊢ (M N)[σ] ≈ M[σ] N[σ] : B[σ,,N[σ]] }} )
 | wf_exp_eq_pi_beta :
   `( forall (r : Ru_pi P s1 s2 s3),
         {{ Γ ⊢ A : Sort@s1 }} ->
-        {{ Γ, A@s1 ⊢ B : Sort@s2 }} ->
-        {{ Γ, A@s1 ⊢ M : B }} ->
+        {{ Γ, A ⊢ B : Sort@s2 }} ->
+        {{ Γ, A ⊢ M : B }} ->
         {{ Γ ⊢ N : A }} ->
         {{ Γ ⊢ (λ r A B M) N ≈ M[Id,,N] : B[Id,,N] }} )
 | wf_exp_eq_pi_eta :
   `( forall (r : Ru_pi P s1 s2 s3),
         {{ Γ ⊢ A : Sort@s1 }} ->
-        {{ Γ, A@s1 ⊢ B : Sort@s2 }} ->
+        {{ Γ, A ⊢ B : Sort@s2 }} ->
         {{ Γ ⊢ M : Π r A B }} ->
         {{ Γ ⊢ M ≈ λ r A B (M[Wk] #0) : Π r A B }} )
 
@@ -233,38 +233,38 @@ with wf_exp_eq {P : PtsSig} : ctx P -> typ P -> exp P -> exp P -> Prop :=
         {{ Γ ⊢ succ M ≈ succ M' : ℕ}} )
 | wf_exp_eq_natrec_cong :
   `( forall (r : Ru_nat P s),
-        {{ Γ, ℕ@s ⊢ A : Sort@s' }} ->
-        {{ Γ, ℕ@s ⊢ A' : Sort@s' }} ->
-        {{ Γ, ℕ@s ⊢ A ≈ A' : Sort@s' }} ->
+        {{ Γ, ℕ ⊢ A : Sort@s' }} ->
+        {{ Γ, ℕ ⊢ A' : Sort@s' }} ->
+        {{ Γ, ℕ ⊢ A ≈ A' : Sort@s' }} ->
         {{ Γ ⊢ MZ ≈ MZ' : A[Id,,zero] }} ->
-        {{ Γ, ℕ@s, A@s' ⊢ MS ≈ MS' : A[Wk∘Wk,,succ #1] }} ->
+        {{ Γ, ℕ, A ⊢ MS ≈ MS' : A[Wk∘Wk,,succ #1] }} ->
         {{ Γ ⊢ M ≈ M' : ℕ}} ->
         {{ Γ ⊢ rec M return A | zero -> MZ | succ -> MS end ≈ rec M' return A' | zero -> MZ' | succ -> MS' end : A[Id,,M] }} )
 | wf_exp_eq_natrec_sub :
   `( forall (r : Ru_nat P s),
         {{ Γ ⊢s σ : Δ }} ->
-        {{ Δ, ℕ@s ⊢ A : Sort@s' }} ->
+        {{ Δ, ℕ ⊢ A : Sort@s' }} ->
         {{ Δ ⊢ MZ : A[Id,,zero] }} ->
-        {{ Δ, ℕ@s, A@s' ⊢ MS : A[Wk∘Wk,,succ #1] }} ->
+        {{ Δ, ℕ, A ⊢ MS : A[Wk∘Wk,,succ #1] }} ->
         {{ Δ ⊢ M : ℕ}} ->
         {{ Γ ⊢ rec M return A | zero -> MZ | succ -> MS end[σ] ≈ rec M[σ] return A[q σ] | zero -> MZ[σ] | succ -> MS[q (q σ)] end : A[σ,,M[σ]] }} )
 | wf_exp_eq_nat_beta_zero :
   `( forall (r : Ru_nat P s),
-        {{ Γ, ℕ@s ⊢ A : Sort@s' }} ->
+        {{ Γ, ℕ ⊢ A : Sort@s' }} ->
         {{ Γ ⊢ MZ : A[Id,,zero] }} ->
-        {{ Γ, ℕ@s, A@s' ⊢ MS : A[Wk∘Wk,,succ #1] }} ->
+        {{ Γ, ℕ, A ⊢ MS : A[Wk∘Wk,,succ #1] }} ->
         {{ Γ ⊢ rec zero return A | zero -> MZ | succ -> MS end ≈ MZ : A[Id,,zero] }} )
 | wf_exp_eq_nat_beta_succ :
   `( forall (r : Ru_nat P s),
-        {{ Γ, ℕ@s ⊢ A : Sort@s' }} ->
+        {{ Γ, ℕ ⊢ A : Sort@s' }} ->
         {{ Γ ⊢ MZ : A[Id,,zero] }} ->
-        {{ Γ, ℕ@s, A@s' ⊢ MS : A[Wk∘Wk,,succ #1] }} ->
+        {{ Γ, ℕ, A ⊢ MS : A[Wk∘Wk,,succ #1] }} ->
         {{ Γ ⊢ M : ℕ}} ->
         {{ Γ ⊢ rec succ M return A | zero -> MZ | succ -> MS end ≈ MS[Id,,M,,rec M return A | zero -> MZ | succ -> MS end] : A[Id,,succ M] }} )
 
 | wf_exp_eq_var :
   `( {{ ⊢ Γ }} ->
-     {{ #x : A@s ∈ Γ }} ->
+     {{ #x : A ∈ Γ }} ->
      {{ Γ ⊢ #x ≈ #x : A }} )
 | wf_exp_eq_var_0_sub :
   `( {{ Γ ⊢s σ : Δ }} ->
@@ -275,12 +275,12 @@ with wf_exp_eq {P : PtsSig} : ctx P -> typ P -> exp P -> exp P -> Prop :=
   `( {{ Γ ⊢s σ : Δ }} ->
      {{ Δ ⊢ A : Sort@s }} ->
      {{ Γ ⊢ M : A[σ] }} ->
-     {{ #x : B@s' ∈ Δ }} ->
+     {{ #x : B ∈ Δ }} ->
      {{ Γ ⊢ #(S x)[σ,,M] ≈ #x[σ] : B[σ] }} )
 | wf_exp_eq_var_weaken :
-  `( {{ ⊢ Γ, B@s' }} ->
-     {{ #x : A@s ∈ Γ }} ->
-     {{ Γ, B@s' ⊢ #x[Wk] ≈ #(S x) : A[Wk] }} )
+  `( {{ ⊢ Γ, B }} ->
+     {{ #x : A ∈ Γ }} ->
+     {{ Γ, B ⊢ #x[Wk] ≈ #(S x) : A[Wk] }} )
 | wf_exp_eq_sub_cong_typ :
   `( {{ Δ ⊢ A }} ->
      {{ Δ ⊢ M ≈ M' : A }} ->
@@ -314,8 +314,8 @@ with wf_sub_eq {P : PtsSig} : ctx P -> ctx P -> sub P -> sub P -> Prop :=
   `( {{ ⊢ Γ }} ->
      {{ Γ ⊢s Id ≈ Id : Γ }} )
 | wf_sub_eq_weaken :
-  `( {{ ⊢ Γ, A@s }} ->
-     {{ Γ, A@s ⊢s Wk ≈ Wk : Γ }} )
+  `( {{ ⊢ Γ, A }} ->
+     {{ Γ, A ⊢s Wk ≈ Wk : Γ }} )
 | wf_sub_eq_compose_cong :
   `( {{ Γ ⊢s τ ≈ τ' : Γ' }} ->
      {{ Γ' ⊢s σ ≈ σ' : Γ'' }} ->
@@ -324,7 +324,7 @@ with wf_sub_eq {P : PtsSig} : ctx P -> ctx P -> sub P -> sub P -> Prop :=
   `( {{ Γ ⊢s σ ≈ σ' : Δ }} ->
      {{ Δ ⊢ A : Sort@s }} ->
      {{ Γ ⊢ M ≈ M' : A[σ] }} ->
-     {{ Γ ⊢s σ,,M ≈ σ',,M' : Δ, A@s }} )
+     {{ Γ ⊢s σ,,M ≈ σ',,M' : Δ, A }} )
 | wf_sub_eq_id_compose_right :
   `( {{ Γ ⊢s σ : Δ }} ->
      {{ Γ ⊢s Id∘σ ≈ σ : Δ }} )
@@ -341,15 +341,15 @@ with wf_sub_eq {P : PtsSig} : ctx P -> ctx P -> sub P -> sub P -> Prop :=
      {{ Γ'' ⊢ A : Sort@s }} ->
      {{ Γ' ⊢ M : A[σ] }} ->
      {{ Γ ⊢s τ : Γ' }} ->
-     {{ Γ ⊢s (σ,,M)∘τ ≈ (σ∘τ),,M[τ] : Γ'', A@s }} )
+     {{ Γ ⊢s (σ,,M)∘τ ≈ (σ∘τ),,M[τ] : Γ'', A }} )
 | wf_sub_eq_p_extend :
   `( {{ Γ' ⊢s σ : Γ }} ->
      {{ Γ ⊢ A : Sort@s }} ->
      {{ Γ' ⊢ M : A[σ] }} ->
      {{ Γ' ⊢s Wk∘(σ,,M) ≈ σ : Γ }} )
 | wf_sub_eq_extend :
-  `( {{ Γ' ⊢s σ : Γ, A@s }} ->
-     {{ Γ' ⊢s σ ≈ (Wk∘σ),,#0[σ] : Γ, A@s }} )
+  `( {{ Γ' ⊢s σ : Γ, A }} ->
+     {{ Γ' ⊢s σ ≈ (Wk∘σ),,#0[σ] : Γ, A }} )
 | wf_sub_eq_sym :
   `( {{ Γ ⊢s σ ≈ σ' : Δ }} ->
      {{ Γ ⊢s σ' ≈ σ : Δ }} )
@@ -382,9 +382,9 @@ with wf_subtyp {P : PtsSig} : ctx P -> typ P -> typ P -> Prop :=
         {{ Γ ⊢ A : Sort@s1 }} ->
         {{ Γ ⊢ A' : Sort@s1 }} ->
         {{ Γ ⊢ A ≈ A' : Sort@s1 }} ->
-        {{ Γ, A@s1 ⊢ B : Sort@s2 }} ->
-        {{ Γ, A'@s1 ⊢ B' : Sort@s2 }} ->
-        {{ Γ, A'@s1 ⊢ B ⊆ B' }} ->
+        {{ Γ, A ⊢ B : Sort@s2 }} ->
+        {{ Γ, A' ⊢ B' : Sort@s2 }} ->
+        {{ Γ, A' ⊢ B ⊆ B' }} ->
         {{ Γ ⊢ Π r A B ⊆ Π r A' B' }} )
 where "Γ ⊢ A ⊆ A'" := (wf_subtyp Γ A A') (in custom judg) : type_scope
 
